src/compiler_generic/toy_example/embedding/core/Floor1_infra.thy
@@ -49,17 +49,17 @@ definition "print_infra_datatype_class = start_map'' O.datatype o (\<lambda>expr
   (\<lambda>isub_name name _ l_attr l_inherited l_cons.
     let (l_attr, l_inherited) = base_attr' (l_attr, of_inh l_inherited)
       ; map_ty = L.map ((\<lambda>x. Typ_apply (Typ_base \<open>option\<close>) [str_hol_of_ty_all Typ_apply Typ_base x]) o snd) in
-    [ Datatype
+    [ Datatype'
         (isub_name datatype_ext_name)
         (  (L.rev_map (\<lambda>x. ( datatype_ext_constr_name @@ mk_constr_name name x
                          , [Raw (datatype_name @@ String.isub x)])) (of_sub l_cons))
         @@@@ [(isub_name datatype_ext_constr_name, Raw const_oid # L.maps map_ty l_inherited)])
-    , Datatype
+    , Datatype'
         (isub_name datatype_name)
         [ (isub_name datatype_constr_name, Raw (isub_name datatype_ext_name) # map_ty l_attr ) ] ]) expr)"
 
 definition "print_infra_datatype_universe expr = start_map O.datatype
-  [ Datatype \<open>\<AA>\<close>
+  [ Datatype' \<open>\<AA>\<close>
       (map_class (\<lambda>isub_name _ _ _ _ _. (isub_name datatype_in, [Raw (isub_name datatype_name)])) expr) ]"
 
 definition "print_infra_type_synonym_class_higher expr = start_map O.type_synonym
